src/impl/TLS13.Impl.Server.Send.fsti
@@ -605,6 +605,7 @@ fn process_send_certificate_verify_serialized
                  'st0.CS.cs_model.CS.model_config.CS.config_role ==
                    CS.ServerEndpoint /\
                  'st0.CS.cs_model.CS.model_handshake.CS.hs_certificate <> None /\
+                 'st0.CS.cs_model.CS.model_handshake.CS.hs_certificate_verify_verified /\
                  Some?
                    'st0.CS.cs_model.CS.model_handshake.CS.hs_keys.CS.ks_server_handshake_traffic /\
                  U64.fits
@@ -666,6 +667,7 @@ fn process_send_stored_certificate_verify_serialized
                   'st0.CS.cs_model.CS.model_config.CS.config_role ==
                     CS.ServerEndpoint /\
                   'st0.CS.cs_model.CS.model_handshake.CS.hs_certificate <> None /\
+                  'st0.CS.cs_model.CS.model_handshake.CS.hs_certificate_verify_verified /\
                   Some?
                     'st0.CS.cs_model.CS.model_handshake.CS.hs_keys.CS.ks_server_handshake_traffic /\
                   U64.fits
